---
publish: true
tags: []
aliases: 
finished: true
title: 题4
created: "2024-10-04 14:09"
updated: "2024-12-09 02:46"
---
## 题4
### 题目
> [!question]+
> 设函数 $f( t)$ 连续,令 $F( {x, y}) = {\int }_{0}^{x - y}( {x - y - t}) f( t) \mathrm{d}t$ ,则 ( )
> (A) $\frac{\partial F}{\partial x} = \frac{\partial F}{\partial y},\frac{{\partial }^{2}F}{\partial {x}^{2}} = \frac{{\partial }^{2}F}{\partial {y}^{2}}$ . 
> (B) $\frac{\partial F}{\partial x} = \frac{\partial F}{\partial y},\frac{{\partial }^{2}F}{\partial {x}^{2}} = - \frac{{\partial }^{2}F}{\partial {y}^{2}}$ .
> (C) $\frac{\partial F}{\partial x} = - \frac{\partial F}{\partial y},\frac{{\partial }^{2}F}{\partial {x}^{2}} = \frac{{\partial }^{2}F}{\partial {y}^{2}}$ . 
> (D) $\frac{\partial F}{\partial x} = - \frac{\partial F}{\partial y},\frac{{\partial }^{2}F}{\partial {x}^{2}} = - \frac{{\partial }^{2}F}{\partial {y}^{2}}$ .
### 分析
> [!NOTE]+
> ![](https://img.hwenyi.tech/202412081413698.webp)
### 解
> [!done]-
> 解 整理 $F( {x, y})$ 的表达式.
> 
> $$
> F( {x, y}) = {\int }_{0}^{x - y}( {x - y - t}) f( t) \mathrm{d}t = ( {x - y}) {\int }_{0}^{x - y}f( t) \mathrm{d}t - {\int }_{0}^{x - y}{tf}( t) \mathrm{d}t.
> $$
> 
> 分别计算 $\frac{\partial F}{\partial x},\frac{{\partial }^{2}F}{\partial {x}^{2}},\frac{\partial F}{\partial y},\frac{{\partial }^{2}F}{\partial {y}^{2}}$ .
> 
> $$
> \frac{\partial F}{\partial x} = ( {x - y}) f( {x - y}) + {\int }_{0}^{x - y}f( t) \mathrm{d}t - ( {x - y}) f( {x - y}) = {\int }_{0}^{x - y}f( t) \mathrm{d}t,
> $$
> 
> $$
> \frac{{\partial }^{2}F}{\partial {x}^{2}} = \frac{\partial \lbrack {{\int }_{0}^{x - y}f( t) \mathrm{d}t}\rbrack }{\partial x} = f( {x - y}) ,
> $$
> 
> $$
> \frac{\partial F}{\partial y} = - ( {x - y}) f( {x - y}) - {\int }_{0}^{x - y}f( t) \mathrm{d}t + ( {x - y}) f( {x - y}) = - {\int }_{0}^{x - y}f( t) \mathrm{d}t,
> $$
> 
> $$
> \frac{{\partial }^{2}F}{\partial {y}^{2}} = \frac{\partial \lbrack {-{\int }_{0}^{x - y}f( t) \mathrm{d}t}\rbrack }{\partial y} = f( {x - y}) .
> $$
> 
> 因此, $\frac{\partial F}{\partial x} = - \frac{\partial F}{\partial y},\frac{{\partial }^{2}F}{\partial {x}^{2}} = \frac{{\partial }^{2}F}{\partial {y}^{2}}$ . 应选 C.