---
publish: true
tags:
  - 偏怪难
aliases: 
finished: true
title: 例3.14
created: 2024-09-27 13:04
updated: 2024-10-16 07:54
---
## 例3.14
### 题目
P54 (1) 设 $a$ 为任意常数,计算 ${\lbrack \begin{array}{lll} 0 & 0 & 0 \\ 0 & 1 & a \\ 0 & 0 & 1 \end{array}\rbrack }^{ * }$ ;

(2) 设 $A = \lbrack \begin{array}{lll} 1 & 1 & 1 \\ 1 & 1 & 1 \\ 1 & 1 & 1 \end{array}\rbrack$ ,求矩阵 $B$ ,使得 ${B}^{ * } = A$ .
### 分析
https://www.bilibili.com/video/BV13A4Ze3Em5?t=177.4&p=32
### 解
解(1) 由 ${\mathbf{A}}^{ * }$ 定义知, ${A}_{11} = 1,{A}_{ij}( {i, j \neq 1})$ 均为 0,故 ${\lbrack \begin{array}{lll} 0 & 0 & 0 \\ 0 & 1 & a \\ 0 & 0 & 1 \end{array}\rbrack }^{ * } = \lbrack \begin{array}{lll} 1 & 0 & 0 \\ 0 & 0 & 0 \\ 0 & 0 & 0 \end{array}\rbrack$ .

(2) $\lbrack \begin{array}{ll} \mathbf{A} & {\mathbf{E}}_{3} \\ {\mathbf{E}}_{3} & \mathbf{O} \end{array}\rbrack = \lbrack \begin{array}{llllll} 1 & 1 & 1 & 1 & 0 & 0 \\ 1 & 1 & 1 & 0 & 1 & 0 \\ 1 & 1 & 1 & 0 & 0 & 1 \\ 1 & 0 & 0 & 0 & 0 & 0 \\ 0 & 1 & 0 & 0 & 0 & 0 \\ 0 & 0 & 1 & 0 & 0 & 0 \end{array}\rbrack \rightarrow \lbrack \begin{matrix} 1 & 0 & 0 & 1 & 0 & 0 \\ 0 & 0 & 0 & - 1 & 1 & 0 \\ 0 & 0 & 0 & - 1 & 0 & 1 \\ 1 & - 1 & - 1 & 0 & 0 & 0 \\ 0 & 1 & 0 & 0 & 0 & 0 \\ 0 & 0 & 1 & 0 & 0 & 0 \end{matrix}\rbrack$ ,

故令 $\mathbf{P} = \lbrack \begin{matrix} 1 & 0 & 0 \\ - 1 & 1 & 0 \\ - 1 & 0 & 1 \end{matrix}\rbrack$ ,则 $\mathbf{P}\mathbf{A}{\mathbf{P}}^{\mathrm{T}} = \lbrack \begin{array}{lll} 1 & 0 & 0 \\ 0 & 0 & 0 \\ 0 & 0 & 0 \end{array}\rbrack$ ,有 $\mathbf{A} = {\mathbf{P}}^{-1}\lbrack \begin{array}{lll} 1 & 0 & 0 \\ 0 & 0 & 0 \\ 0 & 0 & 0 \end{array}\rbrack {( {\mathbf{P}}^{\mathrm{T}}) }^{-1}$ .

又 $r( \mathbf{B}) = 2$ ,则存在可逆矩阵 $\mathbf{Q},\mathbf{R}$ ,有

$$
\mathbf{B} = \mathbf{Q}\lbrack \begin{array}{lll} 0 & 0 & 0 \\ 0 & 1 & a \\ 0 & 0 & 1 \end{array}\rbrack \mathbf{R}
$$

故 ${\mathbf{B}}^{ * } = {\mathbf{R}}^{ * }{\lbrack \begin{array}{lll} 0 & 0 & 0 \\ 0 & 1 & a \\ 0 & 0 & 1 \end{array}\rbrack }^{ * }{\mathbf{Q}}^{ * } = | \mathbf{R}| {\mathbf{R}}^{-1}\lbrack \begin{array}{lll} 1 & 0 & 0 \\ 0 & 0 & 0 \\ 0 & 0 & 0 \end{array}\rbrack | \mathbf{Q}| {\mathbf{Q}}^{-1}$ .

取 $\mathbf{R} = \mathbf{P},\mathbf{Q} = {\mathbf{P}}^{\mathrm{T}}$ ,则 $\mathbf{R}| {{\mathbf{R}}^{-1} = }| \mathbf{P}| {{\mathbf{P}}^{-1} = {\mathbf{P}}^{-1},}| \mathbf{Q}| {{\mathbf{Q}}^{-1} = }| {\mathbf{P}}^{\mathrm{T}}| {\;{( {\mathbf{P}}^{\mathrm{T}}) }^{-1} = {( {\mathbf{P}}^{\mathrm{T}}) }^{-1}}.$ ,即 ${\mathbf{B}}^{ * } = \mathbf{A}$ .

于是 $\mathbf{B} = \mathbf{Q}\lbrack \begin{array}{lll} 0 & 0 & 0 \\ 0 & 1 & a \\ 0 & 0 & 1 \end{array}\rbrack \mathbf{R} = {\mathbf{P}}^{\mathrm{T}}\lbrack \begin{array}{lll} 0 & 0 & 0 \\ 0 & 1 & a \\ 0 & 0 & 1 \end{array}\rbrack \mathbf{P} = \lbrack \begin{matrix} 2 + a & - 1 & - ( {1 + a}) \\ - ( {1 + a}) & 1 & a \\ - 1 & 0 & 1 \end{matrix}\rbrack$ .