## 例3.11
### 题目
P49 设 $\mathrm{A} = {\lbrack \begin{matrix} 0 & 1 & \cdots & 1 \\ 1 & \ddots & \ddots & \vdots \\ \vdots & \ddots & \ddots & 1 \\ 1 & \cdots & 1 & 0 \end{matrix}\rbrack }_{n}$ ,求 ${\mathrm{A}}^{-1}$ .
### 分析
又是这种沿着对角线对称的[[对称矩阵]]，尝试分离出来一个[[秩1矩阵]]+[[对角矩阵]]，然后用[[sherman-morrison公式]]求逆
### 解
设 $\mathrm{A} = -\mathrm{E} + \alpha {\beta }^{\mathrm{T}}$ , 其中 $\alpha  = \begin{pmatrix} 1 \\ \vdots  \\ 1 \end{pmatrix}$, $\beta  = ( 1,1,\cdots ,1 )$ .
由 Sherman-Morrison 公式
$${\mathrm{A}}^{-1} = (-\mathrm{E} + \alpha {\beta }^{\mathrm{T}}{)}^{-1} = (-\mathrm{E}{)}^{-1} - \frac{(-\mathrm{E}{)}^{-1}\alpha {\beta }^{\mathrm{T}}(-\mathrm{E}{)}^{-1}}{1 + {\beta }^{\mathrm{T}}(-\mathrm{E}{)}^{-1}\alpha }$$
注意到 $(-\mathrm{E}{)}^{\mathrm{T}} = -\mathrm{E}$, 则
$$\begin{aligned}
1 + {\beta }^{\mathrm{T}}(-\mathrm{E}{)}^{-1}\alpha  &= 1 + {\beta }^{\mathrm{T}}(-\mathrm{E})\alpha  \\
&= 1 - {\beta }^{\mathrm{T}}\alpha  \\
&= 1 - ( 1,1,\cdots ,1 )\begin{pmatrix} 1 \\ \vdots  \\ 1 \end{pmatrix} \\
&= 1 - n
\end{aligned}$$
所以
$$\begin{aligned}
{\mathrm{A}}^{-1} &= (-\mathrm{E}{)}^{-1} - \frac{(-\mathrm{E}{)}^{-1}\alpha {\beta }^{\mathrm{T}}(-\mathrm{E}{)}^{-1}}{1 - n} \\
&= -\mathrm{E} + \frac{\mathrm{E}\alpha {\beta }^{\mathrm{T}}\mathrm{E}}{n - 1} \\
&= \frac{\alpha {\beta }^{\mathrm{T}}}{n - 1} - \mathrm{E}
\end{aligned}$$
![](https://img.hwenyi.live/202410161322148.webp)
