## 例 9.30
### 题目
P229 设 $f( x) = \{ \begin{array}{ll} {\mathrm{e}}^{-x}, & x \geq 0, \\ 1 + {x}^{2}, & x < 0, \end{array}.$ 则 ${\int }_{-2}^{2}f( {x - 1}) \mathrm{d}x =$
### 分析
![](https://img.hwenyi.tech/202410221911234.webp)
### 解
应填 ${13} - {\mathrm{e}}^{-1}$ 
在积分中作变量代换,令 $x - 1 = t$ ,则
$$
{\int }_{-2}^{2}f( {x - 1}) \mathrm{d}x = {\int }_{-3}^{1}f( t) \mathrm{d}t = {\int }_{-3}^{0}f( t) \mathrm{d}t + {\int }_{0}^{1}f( t) \mathrm{d}t
$$
$$
= {\int }_{-3}^{0}( {1 + {t}^{2}}) \mathrm{d}t + {\int }_{0}^{1}{\mathrm{e}}^{-t}\mathrm{\;d}t = {. ( t + \frac{{t}^{3}}{3}) | }_{-3}^{0} - {. {\mathrm{e}}^{-t}| }_{0}^{1} = {13} - {\mathrm{e}}^{-1}.
$$

