---
TARGET DECK: 刷题::张宇高数强化::第9讲一元函数积分学的计算::例 9.6
---
## 例 9.6
### 题目
Q:P215 (1) 设 $f( x)$ 连续,证明 ${\int }_{0}^{+\infty }f( x) \mathrm{d}x = {\int }_{0}^{+\infty }f( \frac{1}{x}) \frac{1}{{x}^{2}}\mathrm{\;d}x$ ;
(2) 计算 ${\int }_{0}^{+\infty }\frac{1}{1 + {x}^{4}}\mathrm{\;d}x$ 和 ${\int }_{0}^{+\infty }\frac{1}{1 + {x}^{3}}\mathrm{\;d}x$ .
### 分析
A:积分同时出现$\frac{1}{x}$和$x$，要记住这个令$x=\frac{1}{t}$这种手法
### 解
(1)【证】令 $x = \frac{1}{t}$ ,则
$$
{\int }_{0}^{+\infty }f( x) \mathrm{d}x = {\int }_{+\infty }^{0}f( \frac{1}{t}) \mathrm{d}( \frac{1}{t}) = {\int }_{+\infty }^{0}f( \frac{1}{t}) ( {-1}) \frac{1}{{t}^{2}}\mathrm{\;d}t
$$
$$
= {\int }_{0}^{+\infty }f( \frac{1}{t}) \frac{1}{{t}^{2}}\mathrm{\;d}t = {\int }_{0}^{+\infty }f( \frac{1}{x}) \frac{1}{{x}^{2}}\mathrm{\;d}x.
$$
(2)【解】由 (1) 知 ${I}_{1} = {\int }_{0}^{+\infty }\frac{1}{1 + {x}^{4}}\mathrm{\;d}x = {\int }_{0}^{+\infty }\frac{1}{1 + {( \frac{1}{x}) }^{4}} \cdot \frac{1}{{x}^{2}}\mathrm{\;d}x = {\int }_{0}^{+\infty }\frac{{x}^{4}}{1 + {x}^{4}} \cdot \frac{1}{{x}^{2}}\mathrm{\;d}x = {\int }_{0}^{+\infty }\frac{{x}^{2}}{1 + {x}^{4}}\mathrm{\;d}x$ ,所以
$$
{I}_{1} = \frac{1}{2}{\int }_{0}^{+\infty }\frac{1 + {x}^{2}}{1 + {x}^{4}}\mathrm{\;d}x = \frac{1}{2}{\int }_{0}^{+\infty }\frac{1 + \frac{1}{{x}^{2}}}{{x}^{2} + \frac{1}{{x}^{2}}}\mathrm{\;d}x
$$
$$
= \frac{1}{2}{\int }_{0}^{+\infty }\frac{\mathrm{d}( {x - \frac{1}{x}}) }{{( x - \frac{1}{x}) }^{2} + {( \sqrt{2}) }^{2}} = {. \frac{1}{2\sqrt{2}}\arctan \frac{x - \frac{1}{x}}{\sqrt{2}}| }_{0}^{+\infty } = \frac{\sqrt{2}\pi }{4}.
$$
$$
{I}_{2} = {\int }_{0}^{+\infty }\frac{1}{1 + {x}^{3}}\mathrm{\;d}x = {\int }_{0}^{+\infty }\frac{1}{{( \frac{1}{x}) }^{3} + 1} \cdot \frac{1}{{x}^{2}}\mathrm{\;d}x = {\int }_{0}^{+\infty }\frac{{x}^{3}}{1 + {x}^{3}} \cdot \frac{1}{{x}^{2}}\mathrm{\;d}x = {\int }_{0}^{+\infty }\frac{x}{1 + {x}^{3}}\mathrm{\;d}x
$$
故
$$
{I}_{2} = \frac{1}{2}{\int }_{0}^{+\infty }\frac{1 + x}{1 + {x}^{3}}\mathrm{\;d}x = \frac{1}{2}{\int }_{0}^{+\infty }\frac{1}{{x}^{2} - x + 1}\mathrm{\;d}x = \frac{1}{2}{\int }_{0}^{+\infty }\frac{1}{{( x - \frac{1}{2}) }^{2} + {( \frac{\sqrt{3}}{2}) }^{2}}\mathrm{\;d}x
$$
$$
= {. \frac{1}{2}\frac{1}{\frac{\sqrt{3}}{2}}\arctan \frac{x - \frac{1}{2}}{\frac{\sqrt{3}}{2}}| }_{0}^{+\infty } = \frac{1}{\sqrt{3}} \cdot ( {\frac{\pi }{2} + \frac{\pi }{6}}) = \frac{2\sqrt{3}\pi }{9}.
$$

