---
publish: true
tags: 
aliases: 
finished: true
title: 例9.10
created: "2024-09-29 14:33"
updated: "2024-10-21 14:07"
---
## 例9.10
### 题目
P217 求下列不定积分.
(1) $\int {\mathrm{e}}^{x}\sin x\mathrm{\;d}x$ ; 
(2) $\int {\sec }^{3}x\mathrm{\;{dx}}$ ;
(3) $\int \sin ( {\ln x}) {dx}$ 
(4) $\int \sqrt{1 + {x}^{2}}{dx}$
(5) $\int {\sin }^{2}{xdx}$ ;
### 分析
![](https://img.hwenyi.tech/202410212206396.webp)
### 解
【解】(1) $\int {\mathrm{e}}^{x}\sin x\mathrm{\;d}x = \int {\mathrm{e}}^{x}\mathrm{\;d}( {-\cos x}) = - {\mathrm{e}}^{x}\cos x + \int \cos x\mathrm{\;d}( {\mathrm{e}}^{x}) = - {\mathrm{e}}^{x}\cos x + \int {\mathrm{e}}^{x}\mathrm{\;d}( {\sin x})$

$$
= - {\mathrm{e}}^{x}\cos x + {\mathrm{e}}^{x}\sin x - \int {\mathrm{e}}^{x}\sin x\mathrm{\;d}x.
$$

记 $I = \int {\mathrm{e}}^{x}\sin x\mathrm{\;d}x$ ,于是 $I = {\mathrm{e}}^{x}( {\sin x - \cos x}) - I$ ,即 $I = \frac{1}{2}{\mathrm{e}}^{x}( {\sin x - \cos x}) + C$ .

【注】本积分也可利用 $\int {\mathrm{e}}^{ax}\sin {bx}\mathrm{\;d}x = \frac{| \begin{matrix} {( {\mathrm{e}}^{ax}) }^{\prime } & {( \sin bx) }^{\prime } \\ {\mathrm{e}}^{ax} & \sin {bx} \end{matrix}| }{{a}^{2} + {b}^{2}} + C$ 求解,即

$$
\int {\mathrm{e}}^{x}\sin x\mathrm{\;d}x = \frac{| \begin{matrix} {( {\mathrm{e}}^{x}) }^{\prime } & {( \sin x) }^{\prime } \\ {\mathrm{e}}^{x} & \sin x \end{matrix}| }{{1}^{2} + {1}^{2}} + C = \frac{{\mathrm{e}}^{x}\sin x - {\mathrm{e}}^{x}\cos x}{2} + C.
$$

(2) $\int {\sec }^{3}x\mathrm{\;d}x = \int \sec x\mathrm{\;d}( {\tan x}) = \sec x\tan x - \int \sec x{\tan }^{2}x\mathrm{\;d}x$

$$
= \sec x\tan x - \int {\sec }^{3}x\mathrm{\;d}x + \int \sec x\mathrm{\;d}x = \sec x\tan x - \int {\sec }^{3}x\mathrm{\;d}x + \ln | {\sec x + \tan x}| .
$$

记 $I = \int {\sec }^{3}x\mathrm{\;d}x, I = \sec x\tan x - I + \ln | {\sec x + \tan x}|$ ,即

$$
I = \frac{1}{2}\sec x\tan x + \frac{1}{2}\ln | {\sec x + \tan x}| + C.
$$

(3) 记 $I = \int \sin ( {\ln x}) \mathrm{d}x = x\sin ( {\ln x}) - \int x\mathrm{\;d}\lbrack {\sin ( {\ln x}) }\rbrack$

$$
= x\sin ( {\ln x}) - \int x\cos ( {\ln x}) \frac{\mathrm{d}x}{x} = x\sin ( {\ln x}) - \int \cos ( {\ln x}) \mathrm{d}x
$$

$$
= x\sin ( {\ln x}) - x\cos ( {\ln x}) + \int x\mathrm{\;d}\lbrack {\cos ( {\ln x}) }\rbrack = x\sin ( {\ln x}) - x\cos ( {\ln x}) - \int x\sin ( {\ln x}) \frac{\mathrm{d}x}{x}
$$

$$
= x\sin ( {\ln x}) - x\cos ( {\ln x}) - I.
$$

于是 $I = \frac{x}{2}\lbrack {\sin ( {\ln x}) - \cos ( {\ln x}) }\rbrack + C$ .

(4) $\int \sqrt{1 + {x}^{2}}\mathrm{\;d}x = x\sqrt{1 + {x}^{2}} - \int \frac{{x}^{2}}{\sqrt{1 + {x}^{2}}}\mathrm{\;d}x = x\sqrt{1 + {x}^{2}} - \int \sqrt{1 + {x}^{2}}\mathrm{\;d}x + \int \frac{1}{\sqrt{1 + {x}^{2}}}\mathrm{\;d}x$

$$
= x\sqrt{1 + {x}^{2}} - \int \sqrt{1 + {x}^{2}}\mathrm{\;d}x + \ln ( {x + \sqrt{{x}^{2} + 1}}) .
$$

记 $I = \int \sqrt{1 + {x}^{2}}\mathrm{\;d}x$ ,于是 $I = x\sqrt{1 + {x}^{2}} - I + \ln ( {x + \sqrt{{x}^{2} + 1}})$ ,即

$$
I = \frac{x}{2}\sqrt{1 + {x}^{2}} + \frac{1}{2}\ln ( {x + \sqrt{{x}^{2} + 1}}) + C.
$$

(5) 因为
$$
I = \int {\sin }^{2}x\mathrm{\;d}x = - \int \sin x\mathrm{\;d}( {\cos x}) = - \sin x\cos x + \int {\cos }^{2}x\mathrm{\;d}x
$$

$$
= - \sin x\cos x + \int ( {1 - {\sin }^{2}x}) \mathrm{d}x = - \sin x\cos x + x - I,
$$

所以 $I = \frac{1}{2}( {x - \sin x\cos x}) + C$ .

【注】用 ${\sin }^{2}x = \frac{1 - \cos {2x}}{2}$ 亦可.
