---
publish: true
tags: []
aliases: 
finished: true
title: 题6
created: "2024-10-04 13:46"
updated: "2024-12-01 06:54"
---
## 题6
### 题目
> [!question]+
> 已知函数 $f( {x, y}) = \frac{{\mathrm{e}}^{x}}{x - y}$ ,则 ( )
> (A) ${f}_{x}^{\prime } - {f}_{y}^{\prime } = 0$ .
> (B) ${f}_{x}^{\prime } + {f}_{y}^{\prime } = 0$ . 
> (C) ${f}_{x}^{\prime } - {f}_{y}^{\prime } = f$ . 
> (D) ${f}_{x}^{\prime } + {f}_{y}^{\prime } = f$ .
### 分析
> [!NOTE]+
> ![](https://img.hwenyi.live/202411291621156.webp)
### 解
> [!done]-
> 解 分别计算 ${f}_{x}^{\prime },{f}_{y}^{\prime }$ 得
> 
> $$
> {f}_{x}^{\prime } = \frac{{\mathrm{e}}^{x}( {x - y}) - {\mathrm{e}}^{x}}{{( x - y) }^{2}},\;{f}_{y}^{\prime } = \frac{{\mathrm{e}}^{x}}{{( x - y) }^{2}}.
> $$
> 
> 因此,
> 
> $$
> {f}_{x}^{\prime } + {f}_{y}^{\prime } = \frac{{\mathrm{e}}^{x}( {x - y}) }{{( x - y) }^{2}} = \frac{{\mathrm{e}}^{x}}{x - y} = f.
> $$
> 
> 应选 D.