---
publish: true
tags: []
aliases: 
finished: true
title: 题1
created: "2024-10-04 14:12"
updated: "2024-12-09 08:44"
---
## 题1
### 题目
> [!question]+
> 曲线 $y = x\ln ( {\mathrm{e} + \frac{1}{x - 1}})$ 的斜渐近线方程为 ( )
> (A) $y = x + \mathrm{e}$ . 
> (B) $y = x + \frac{1}{\mathrm{e}}$ .
> (C) $y = x$ . 
> (D) $y = x - \frac{1}{\mathrm{e}}$ .
### 分析
> [!NOTE]+
> 这题我们也做过：[[例5.13]]
> ![](https://img.hwenyi.tech/202412091644739.webp)
### 解
> [!done]-
> 解 先计算 $\mathop{\lim }\limits_{{x \rightarrow \infty }}\frac{y}{x}$ .
> 
> $$
> \mathop{\lim }\limits_{{x \rightarrow \infty }}\frac{y}{x} = \mathop{\lim }\limits_{{x \rightarrow \infty }}\frac{x\ln ( {\mathrm{e} + \frac{1}{x - 1}}) }{x} = \mathop{\lim }\limits_{{x \rightarrow \infty }}\ln ( {\mathrm{e} + \frac{1}{x - 1}}) = 1.
> $$
> 
> 由此可得斜渐近线的斜率为 1 .
> 
> 下面计算 $\mathop{\lim }\limits_{{x \rightarrow \infty }}( {y - x})$ .
> 
> $$
> \mathop{\lim }\limits_{{x \rightarrow \infty }}( {y - x}) = \mathop{\lim }\limits_{{x \rightarrow \infty }}\lbrack {x\ln ( {\mathrm{e} + \frac{1}{x - 1}}) - x}\rbrack = \mathop{\lim }\limits_{{x \rightarrow \infty }}x\lbrack {\ln ( {\mathrm{e} + \frac{1}{x - 1}}) - 1}\rbrack
> $$
> 
> $$
> = \mathop{\lim }\limits_{{x \rightarrow \infty }}x\lbrack {\ln ( {\mathrm{e} + \frac{1}{x - 1}}) - \ln \mathrm{e}}\rbrack = \mathop{\lim }\limits_{{x \rightarrow \infty }}x\ln \lbrack {1 + \frac{1}{\mathrm{e}( {x - 1}) }}\rbrack
> $$
> 
> $$
> \frac{\ln \lbrack {1 + \frac{1}{\mathrm{e}( {x - 1}) }}\rbrack \sim \frac{1}{\mathrm{e}( {x - 1}) }}{}\mathop{\lim }\limits_{{x \rightarrow \infty }}x \cdot \frac{1}{\mathrm{e}( {x - 1}) } = \frac{1}{\mathrm{e}}.
> $$
> 
> 因此,曲线 $y = x\ln ( {\mathrm{e} + \frac{1}{x - 1}})$ 的斜渐近线方程为 $y = x + \frac{1}{\mathrm{e}}$ . 应选 B.