---
aliases: 
tags: 
publish: false
finished: true
created: 2024-06-12 17:58
updated: 2024-06-25 15:50
---
## 题2.14
### 题目
设 3 阶方阵 $\mathbf{A},\mathbf{B}$ 满足 ${\mathbf{A}}^{-1}\mathbf{B}\mathbf{A} = 6\mathbf{A} + \mathbf{B}\mathbf{A}$ ,且 $\mathbf{A} = \lbrack  \begin{matrix} \frac{1}{3} & 0 & 0 \\  0 & \frac{1}{4} & 0 \\  0 & 0 & \frac{1}{5} \end{matrix}\rbrack$ ,求 $\mathbf{B}$ .
### 分析
显然 $\mathbf{A}$ 可逆,在方程两端右边乘 ${\mathbf{A}}^{{-}1}$ ,得

$$
{\mathbf{A}}^{{-}1}\mathbf{B} = 6\mathbf{E} + \mathbf{B},
$$

即
$$
( {\mathbf{A}}^{{-}1} {-} \mathbf{E} )\mathbf{B} = 6\mathbf{E},\mathbf{B} = 6{( {\mathbf{A}}^{{-}1} {-} \mathbf{E} )}^{{-}1}.
$$
又
$$
{\mathbf{A}}^{{-}1} = \lbrack \begin{array}{lll} 3 & 0 & 0 \\ 0 & 4 & 0 \\ 0 & 0 & 5 \end{array} \rbrack,{\mathbf{A}}^{{-}1} {-} \mathbf{E} = \lbrack \begin{array}{lll} 2 & 0 & 0 \\ 0 & 3 & 0 \\ 0 & 0 & 4 \end{array} \rbrack,{( {\mathbf{A}}^{{-}1} {-} \mathbf{E} )}^{{-}1} = \lbrack \begin{array}{lll} \frac{1}{2} & 0 & 0 \\ 0 & \frac{1}{3} & 0 \\ 0 & 0 & \frac{1}{4} \end{array} \rbrack,
$$

故
$$
\mathbf{B} = 6{( {\mathbf{A}}^{{-}1} {-} \mathbf{E} )}^{{-}1} = \lbrack \begin{array}{lll} 3 & 0 & 0 \\ 0 & 2 & 0 \\ 0 & 0 & \frac{3}{2} \end{array} \rbrack.
$$
### 解
![](https://img.hwenyi.live/202409041441565.webp)
