## 题6.2
### 题目
化二次型 $f( {{x}_{1},{x}_{2},{x}_{3}})  = {x}_{1}^{2} + 2{x}_{1}{x}_{2} + 2{x}_{1}{x}_{3} - {x}_{2}^{2} - 2{x}_{2}{x}_{3} - {x}_{3}^{2}$ 为标准形,并写出所作的可逆线性变换.
### 分析 
配方法：提取平方项一起，使非平方项为零.
### 解 
![](https://img.hwenyi.tech/202409061700523.webp)
$$
\begin{aligned}
f(x_1,x_2,x_3)&=x_1^2+2x_1x_2+2x_1x_3-x_2^2-2x_2x_3-x_3^2 \\
&=(x_1+x_2)^2-2x_2^2-2x_2x_3+2x_1x_3 \\
&=(x_1+x_2+x_3)^2-2x_2(x_2+x_3)+x_3^2 \\
&=(x_1+x_2+x_3)^2-2(x_2+\frac{1}{2}x_3)^2+\frac{1}{2}x_3^2 \\
&=y_1^2-2y_2^2+\frac{1}{2}y_3^2
\end{aligned}
$$
其中
$$
\begin{cases}
y_1 = x_1+x_2+x_3 \\
y_2 = x_2+\frac{1}{2}x_3 \\
y_3 = x_3
\end{cases}
\qquad
\Rightarrow
\qquad
\begin{cases}
x_1 = y_1-y_2-y_3 \\
x_2 = y_2-\frac{1}{2}y_3 \\
x_3 = y_3
\end{cases}
$$
写成矩阵形式：
$$
X=CY,\qquad
C=
\begin{bmatrix}
1 & -1 & -1 \\
0 & 1 & -\frac{1}{2} \\
0 & 0 & 1
\end{bmatrix}
$$
由于
$$
|C|=
\begin{vmatrix}
1 & -1 & -1 \\
0 & 1 & -\frac{1}{2} \\
0 & 0 & 1
\end{vmatrix}
=1\neq 0,
$$
所以该线性变换可逆.

