## 例 9.31
### 题目
P229 设 $f( x) = \{ \begin{array}{l} {2x} + \frac{3}{2}{x}^{2}, - 1 \leq x < 0, \\ \frac{x{\mathrm{e}}^{x}}{{( {\mathrm{e}}^{x} + 1) }^{2}},0 \leq x \leq 1, \end{array}.$ 求函数 $F( x) = {\int }_{-1}^{x}f( t) \mathrm{d}t$ 的表达式.
### 分析
分段讨论计算即可
### 解
【解】当 $x \in \lbrack - 1,0)$ 时,

$$
F( x) = {\int }_{-1}^{x}f( t) \mathrm{d}t = {\int }_{-1}^{x}( {{2t} + \frac{3}{2}{t}^{2}}) \mathrm{d}t = {. ( {t}^{2} + \frac{1}{2}{t}^{3}) | }_{-1}^{x} = \frac{1}{2}{x}^{3} + {x}^{2} - \frac{1}{2};
$$

当 $x \in \lbrack {0,1}\rbrack$ 时,

$$
F( x) = {\int }_{-1}^{x}f( t) \mathrm{d}t = {\int }_{-1}^{0}f( t) \mathrm{d}t + {\int }_{0}^{x}f( t) \mathrm{d}t = {. ( {t}^{2} + \frac{1}{2}{t}^{3}) | }_{-1}^{0} + {\int }_{0}^{x}\frac{t{\mathrm{e}}^{t}}{{( {\mathrm{e}}^{t} + 1) }^{2}}\mathrm{\;d}t
$$

$$
= - \frac{1}{2} + {\int }_{0}^{x}( {-t}) \mathrm{d}( \frac{1}{{\mathrm{e}}^{t} + 1}) = - {. \frac{1}{2} - \frac{t}{{\mathrm{e}}^{t} + 1}| }_{0}^{x} + {\int }_{0}^{x}\frac{\mathrm{d}t}{{\mathrm{e}}^{t} + 1}
$$

$$
= - \frac{1}{2} - \frac{x}{{\mathrm{e}}^{x} + 1} + {\int }_{0}^{x}\frac{\mathrm{d}( {\mathrm{e}}^{t}) }{{\mathrm{e}}^{t}( {{\mathrm{e}}^{t} + 1}) } = - \frac{1}{2} - \frac{x}{{\mathrm{e}}^{x} + 1} + {\int }_{0}^{x}( {\frac{1}{{\mathrm{e}}^{t}} - \frac{1}{{\mathrm{e}}^{t} + 1}}) \mathrm{d}( {\mathrm{e}}^{t})
$$

$$
= - {. \frac{1}{2} - \frac{x}{{\mathrm{e}}^{x} + 1} + \ln \frac{{\mathrm{e}}^{t}}{{\mathrm{e}}^{t} + 1}| }_{0}^{x} = - \frac{1}{2} - \frac{x}{{\mathrm{e}}^{x} + 1} + \ln \frac{{\mathrm{e}}^{x}}{{\mathrm{e}}^{x} + 1} - \ln \frac{1}{2},
$$

所以
$$
F( x) = \{ \begin{array}{ll} \frac{{x}^{3}}{2} + {x}^{2} - \frac{1}{2}, & - 1 \leq x < 0, \\ \ln \frac{{\mathrm{e}}^{x}}{{\mathrm{e}}^{x} + 1} - \frac{x}{{\mathrm{e}}^{x} + 1} + \ln 2 - \frac{1}{2}, & 0 \leq x \leq 1. \end{array}.
$$