## 例9.15
### 题目
P220 求不定积分 $\int \frac{{x}^{3} + 1}{{x}^{3} - 5{x}^{2} + {6x}}\mathrm{\;d}x$ .
### 分析
上下次数一致，考虑先分离常数，把上面的次数降低一次，在根据[[部分分式积分法]]进行计算。 
### 解
【解】 $\frac{{x}^{3} + 1}{{x}^{3} - 5{x}^{2} + {6x}} = 1 + \frac{5{x}^{2} - {6x} + 1}{{x}^{3} - 5{x}^{2} + {6x}}$ . 由于 ${x}^{3} - 5{x}^{2} + {6x} = x( {x - 2}) ( {x - 3})$ ,故可设

$$
\frac{5{x}^{2} - {6x} + 1}{{x}^{3} - 5{x}^{2} + {6x}} = \frac{A}{x} + \frac{B}{x - 2} + \frac{C}{x - 3},
$$

即
$$
\frac{5{x}^{2} - {6x} + 1}{{x}^{3} - 5{x}^{2} + {6x}} = \frac{A( {x - 2}) ( {x - 3}) + {Bx}( {x - 3}) + {Cx}( {x - 2}) }{{x}^{3} - 5{x}^{2} + {6x}},
$$

所以
$$
5{x}^{2} - {6x} + 1 = A( {x - 2}) ( {x - 3}) + {Bx}( {x - 3}) + {Cx}( {x - 2}) .
$$

令 $x = 0$ ,得 ${6A} = 1$ ,即 $A = \frac{1}{6}$ ; 令 $x = 2$ ,得 $- {2B} = 9$ ,即 $B = - \frac{9}{2}$ ; 令 $x = 3$ ,得 ${3C} = {28}$ ,即 $C = \frac{28}{3}$ . 所以

$$
\int \frac{{x}^{3} + 1}{{x}^{3} - 5{x}^{2} + {6x}}\mathrm{\;d}x = \int ( {1 + \frac{1}{6x} - \frac{9}{2} \cdot \frac{1}{x - 2} + \frac{28}{3} \cdot \frac{1}{x - 3}}) \mathrm{d}x = x + \frac{1}{6}\ln | x| - \frac{9}{2}\ln | {x - 2}| + \frac{28}{3}\ln | {x - 3}| + C.
$$