---
publish: true
tags: []
aliases: 
finished: true
title: 题4
created: "2024-10-04 14:09"
updated: "2024-12-09 02:46"
---
## 题4
### 题目
> [!question]+
> 设函数 $f\left( t\right)$ 连续,令 $F\left( {x, y}\right) = {\int }_{0}^{x - y}\left( {x - y - t}\right) f\left( t\right) \mathrm{d}t$ ,则 ( )
> (A) $\frac{\partial F}{\partial x} = \frac{\partial F}{\partial y},\frac{{\partial }^{2}F}{\partial {x}^{2}} = \frac{{\partial }^{2}F}{\partial {y}^{2}}$ . 
> (B) $\frac{\partial F}{\partial x} = \frac{\partial F}{\partial y},\frac{{\partial }^{2}F}{\partial {x}^{2}} = - \frac{{\partial }^{2}F}{\partial {y}^{2}}$ .
> (C) $\frac{\partial F}{\partial x} = - \frac{\partial F}{\partial y},\frac{{\partial }^{2}F}{\partial {x}^{2}} = \frac{{\partial }^{2}F}{\partial {y}^{2}}$ . 
> (D) $\frac{\partial F}{\partial x} = - \frac{\partial F}{\partial y},\frac{{\partial }^{2}F}{\partial {x}^{2}} = - \frac{{\partial }^{2}F}{\partial {y}^{2}}$ .
### 分析
> [!NOTE]+
> ![](https://img.hwenyi.live/202412081413698.webp)
### 解
> [!done]-
> 解 整理 $F\left( {x, y}\right)$ 的表达式.
> 
> $$
> F\left( {x, y}\right) = {\int }_{0}^{x - y}\left( {x - y - t}\right) f\left( t\right) \mathrm{d}t = \left( {x - y}\right) {\int }_{0}^{x - y}f\left( t\right) \mathrm{d}t - {\int }_{0}^{x - y}{tf}\left( t\right) \mathrm{d}t.
> $$
> 
> 分别计算 $\frac{\partial F}{\partial x},\frac{{\partial }^{2}F}{\partial {x}^{2}},\frac{\partial F}{\partial y},\frac{{\partial }^{2}F}{\partial {y}^{2}}$ .
> 
> $$
> \frac{\partial F}{\partial x} = \left( {x - y}\right) f\left( {x - y}\right) + {\int }_{0}^{x - y}f\left( t\right) \mathrm{d}t - \left( {x - y}\right) f\left( {x - y}\right) = {\int }_{0}^{x - y}f\left( t\right) \mathrm{d}t,
> $$
> 
> $$
> \frac{{\partial }^{2}F}{\partial {x}^{2}} = \frac{\partial \left\lbrack {{\int }_{0}^{x - y}f\left( t\right) \mathrm{d}t}\right\rbrack }{\partial x} = f\left( {x - y}\right) ,
> $$
> 
> $$
> \frac{\partial F}{\partial y} = - \left( {x - y}\right) f\left( {x - y}\right) - {\int }_{0}^{x - y}f\left( t\right) \mathrm{d}t + \left( {x - y}\right) f\left( {x - y}\right) = - {\int }_{0}^{x - y}f\left( t\right) \mathrm{d}t,
> $$
> 
> $$
> \frac{{\partial }^{2}F}{\partial {y}^{2}} = \frac{\partial \left\lbrack {-{\int }_{0}^{x - y}f\left( t\right) \mathrm{d}t}\right\rbrack }{\partial y} = f\left( {x - y}\right) .
> $$
> 
> 因此, $\frac{\partial F}{\partial x} = - \frac{\partial F}{\partial y},\frac{{\partial }^{2}F}{\partial {x}^{2}} = \frac{{\partial }^{2}F}{\partial {y}^{2}}$ . 应选 C.