---
publish: true
tags: []
aliases: 
finished: true
title: 题10
created: "2024-10-04 13:49"
updated: "2024-12-01 06:54"
---
## 题10
### 题目
> [!question]+
> (10) 设函数 $y = y\left( x\right)$ 由参数方程 $\left\{ \begin{array}{l} x = t + {\mathrm{e}}^{t}, \\ y = \sin t \end{array}\right.$ 确定,则 ${\left. \frac{{\mathrm{d}}^{2}y}{\mathrm{\;d}{x}^{2}}\right| }_{t = 0} =$
### 分析
> [!NOTE]+
> ![](https://img.hwenyi.live/202411301348449.webp)
### 解
> [!done]-
> 解 根据由参数方程确定的函数的求导公式,
> 
> $$
> \frac{\mathrm{d}y}{\mathrm{\;d}x} = \frac{\mathrm{d}y}{\mathrm{\;d}t}/\frac{\mathrm{d}x}{\mathrm{\;d}t} = \frac{\cos t}{1 + {\mathrm{e}}^{t}},
> $$
> 
> $$
> \frac{{\mathrm{d}}^{2}y}{\mathrm{\;d}{x}^{2}} = \frac{\mathrm{d}\left\lbrack {{y}^{\prime }\left( x\right) }\right\rbrack }{\mathrm{d}t}/\frac{\mathrm{d}x}{\mathrm{\;d}t} = \frac{\frac{\mathrm{d}\left( \frac{\cos t}{1 + {\mathrm{e}}^{t}}\right) }{\mathrm{d}t}}{1 + {\mathrm{e}}^{t}} = \frac{\frac{-\sin t\left( {1 + {\mathrm{e}}^{t}}\right) - \cos t{\mathrm{e}}^{t}}{{\left( 1 + {\mathrm{e}}^{t}\right) }^{2}}}{1 + {\mathrm{e}}^{t}}
> $$
> 
> $$
> = \frac{-\sin t\left( {1 + {\mathrm{e}}^{t}}\right) - \cos t{\mathrm{e}}^{t}}{{\left( 1 + {\mathrm{e}}^{t}\right) }^{3}}.
> $$
> 
> 当 $t = 0$ 时, ${\left. \frac{{\mathrm{d}}^{2}y}{\mathrm{\;d}{x}^{2}}\right| }_{t = 0} = - \frac{1}{8}$ .
> 
> 或者也可以这样计算 $\frac{{\mathrm{d}}^{2}y}{\mathrm{\;d}{x}^{2}}$ .
> 
> 由于 ${x}^{\prime }\left( t\right) = 1 + {\mathrm{e}}^{t},{x}^{\prime \prime }\left( t\right) = {\mathrm{e}}^{t},{y}^{\prime }\left( t\right) = \cos t,{y}^{\prime \prime }\left( t\right) = - \sin t$ ,故
> 
> $$
> \frac{{\mathrm{d}}^{2}y}{\mathrm{\;d}{x}^{2}} = \frac{{y}^{\prime \prime }\left( t\right) {x}^{\prime }\left( t\right) - {y}^{\prime }\left( t\right) {x}^{\prime \prime }\left( t\right) }{{\left\lbrack {x}^{\prime }\left( t\right) \right\rbrack }^{3}} = \frac{-\sin t\left( {1 + {\mathrm{e}}^{t}}\right) - \cos t{\mathrm{e}}^{t}}{{\left( 1 + {\mathrm{e}}^{t}\right) }^{3}}.
> $$