## 例2.12
### 题目
P74 (1) (仅数学一、数学三) 设 ${x}_{n + 1} = \sqrt{{x}_{n}( {{x}_{n} + {a}_{n}}) }( {n = 1,2,\cdots }) ,{x}_{1} = 1$ ,且正项级数 $\mathop{\sum }\limits_{{n = 1}}^{\infty }{a}_{n}$
收敛,证明数列 $\{ {x}_{n}\}$ 收敛;

(2) 设 ${x}_{n + 1} = \frac{{x}_{n}^{2}}{2( {{x}_{n} - 1}) }( {n = 1,2,\cdots }) ,{x}_{1} > 1$ ,证明数列 $\{ {x}_{n}\}$ 收敛,并求 $\mathop{\lim }\limits_{{n \rightarrow \infty }}{x}_{n}$ 
(3) 设 ${x}_{1} > 0,{x}_{n + 1} = \frac{2{x}_{n}^{3} + 1}{3{x}_{n}^{2}}( {n = 1,2,\cdots })$ ,证明数列 $\{ {x}_{n}\}$ 收敛,并求 $\mathop{\lim }\limits_{{n \rightarrow \infty }}{x}_{n}$ .
### 分析
- [02:21](https://www.bilibili.com/video/BV1Yw4m1a757?p=68&t=141.54251#t=02:21.54) 
### 解
(1)【证】由于 ${a}_{n} > 0$ ,故 ${x}_{n + 1} = \sqrt{{x}_{n}( {{x}_{n} + {a}_{n}}) } > {x}_{n}$ ,则 ${x}_{n + 1} - {x}_{n} = \sqrt{{x}_{n}( {{x}_{n} + {a}_{n}}) } - {x}_{n} = \frac{{a}_{n}{x}_{n}}{\sqrt{{x}_{n}( {{x}_{n} + {a}_{n}}) } + {x}_{n}} <$ $\frac{1}{2}{a}_{n}$ ,又 $\mathop{\sum }\limits_{{n = 1}}^{\infty }{a}_{n}$ 收敛,故 $\mathop{\sum }\limits_{{n = 1}}^{\infty }( {{x}_{n + 1} - {x}_{n}})$ 收敛,所以数列 $\{ {x}_{n}\}$ 收敛.
$$
\text{(2)【解】}\;{x}_{n + 1} = \frac{1}{2}( {{x}_{n} - 1 + \frac{1}{{x}_{n} - 1}}) + 1 \geq 2,{x}_{n + 1} - {x}_{n} = \frac{{x}_{n}( {2 - {x}_{n}}) }{2( {{x}_{n} - 1}) } \leq 0\text{,}
$$

故由单调有界准则知,数列 $\{ {x}_{n}\}$ 收敛.
设 $\mathop{\lim }\limits_{{n \rightarrow \infty }}{x}_{n} = A$ ,则有 $A = \frac{{A}^{2}}{2( {A - 1}) }$ ,解得 $A = 2$ 或 $A = 0$ (舍去),故 $\mathop{\lim }\limits_{{n \rightarrow \infty }}{x}_{n} = 2$ .
(3)【解】
$$
{x}_{n + 1} = \frac{1}{3}( {{x}_{n} + {x}_{n} + \frac{1}{{x}_{n}^{2}}}) \geq \sqrt[3]{1} = 1,{x}_{n + 1} - {x}_{n} = \frac{1 - {x}_{n}^{3}}{3{x}_{n}^{2}} \leq 0,
$$
故由单调有界准则知,数列 $\{ {x}_{n}\}$ 收敛.
设 $\mathop{\lim }\limits_{{n \rightarrow \infty }}{x}_{n} = A$ ,则 $A = \frac{2{A}^{3} + 1}{3{A}^{2}}$ ,解得 $A = 1$ ,故 $\mathop{\lim }\limits_{{n \rightarrow \infty }}{x}_{n} = 1$ .
③作商 $\frac{{x}_{n + 1}}{{x}_{n}}$ ( ${x}_{n + 1}$ 与 ${x}_{n}$ 同号),根据与 1 的大小关系定单调.