---
publish: true
tags: []
aliases: 
finished: true
title: 题11
created: "2024-12-06 04:08"
updated: "2024-12-21 12:03"
---
## 题11
### 题目

设二次型 $f(x_1, x_2, x_3)$ 在正交变换 $\mathbf{x} = \mathbf{P}\mathbf{y}$ 下的标准形为 $y_1^2 - 2y_2^2 + 3y_3^2$，其中 $\mathbf{P} = (\mathbf{e}_1, \mathbf{e}_2, \mathbf{e}_3)$。若 $\mathbf{Q} = (\mathbf{e}_2, \mathbf{e}_1, -\mathbf{e}_3)$，则 $f(x_1, x_2, x_3)$ 在正交变换 $\mathbf{x} = \mathbf{Q}\mathbf{y}$ 下的标准形为( )
(A) $-2y_1^2 + y_2^2 + 3y_3^2$. 
(B) $-2y_1^2 + y_2^2 - 3y_3^2$.
(C) $y_1^2 - 2y_2^2 + 3y_3^2$. 
(D) $2y_1^2 + y_2^2 + 3y_3^2$.

### 分析
真题改编：[[刷题/数二真题/2015年数二试题/题8]]
### 解

答案 A.

解 设$f(x_1,x_2,x_3) = x^T A x$，其中$A$是3阶实对称矩阵，$x = (x_1, x_2, x_3)^T$。由题意可知$P^T A P = \text{diag}(1, -2, 3)$。注意到

$$Q = (e_2, e_1, -e_3) = (e_1, e_2, e_3) \begin{pmatrix} 0 & 1 & 0 \\ 1 & 0 & 0 \\ 0 & 0 & -1 \end{pmatrix} = P \begin{pmatrix} 0 & 1 & 0 \\ 1 & 0 & 0 \\ 0 & 0 & -1 \end{pmatrix},$$

故

$$Q^T A Q = \begin{pmatrix} 0 & 1 & 0 \\ 1 & 0 & 0 \\ 0 & 0 & -1 \end{pmatrix} P^T A P \begin{pmatrix} 0 & 1 & 0 \\ 1 & 0 & 0 \\ 0 & 0 & -1 \end{pmatrix} = \begin{pmatrix} 0 & 1 & 0 \\ 1 & 0 & 0 \\ 0 & 0 & -1 \end{pmatrix} \begin{pmatrix} 1 & 0 & 0 \\ 0 & -2 & 0 \\ 0 & 0 & 3 \end{pmatrix} \begin{pmatrix} 0 & 1 & 0 \\ 1 & 0 & 0 \\ 0 & 0 & -1 \end{pmatrix} = \begin{pmatrix} -2 & 0 & 0 \\ 0 & 1 & 0 \\ 0 & 0 & 3 \end{pmatrix}.$$
