---
publish: true
tags: 
aliases: 
finished: true
title: 题12
created: "2024-10-04 14:06"
updated: "2024-12-01 06:54"
---
## 题12
### 题目
> [!question]+
> 设函数 $y = y\left( x\right)$ 由参数方程 $\left\{ \begin{array}{l} x = 2{\mathrm{e}}^{t} + t + 1, \\ y = 4\left( {t - 1}\right) {\mathrm{e}}^{t} + {t}^{2} \end{array}\right.$ 确定,则 ${\left. \frac{{\mathrm{d}}^{2}y}{\mathrm{\;d}{x}^{2}}\right| }_{t = 0} =$
### 分析
> [!NOTE]+
> ![](https://img.hwenyi.live/202412071745509.webp)
### 解
> [!done]-
> 解 根据由参数方程确定的函数的导数计算公式,
> 
> $$
> \frac{\mathrm{d}y}{\mathrm{\;d}x} = \frac{\mathrm{d}y}{\mathrm{\;d}t}/\frac{\mathrm{d}x}{\mathrm{\;d}t} = \frac{4{\mathrm{e}}^{t} + 4\left( {t - 1}\right) {\mathrm{e}}^{t} + {2t}}{2{\mathrm{e}}^{t} + 1} = \frac{{4t}{\mathrm{e}}^{t} + {2t}}{2{\mathrm{e}}^{t} + 1} = {2t}.
> $$
> 
> $$
> \frac{{\mathrm{d}}^{2}y}{\mathrm{\;d}{x}^{2}} = \frac{\mathrm{d}\left( \frac{\mathrm{d}y}{\mathrm{\;d}x}\right) }{\mathrm{d}t}/\frac{\mathrm{d}x}{\mathrm{\;d}t} = \frac{2}{2{\mathrm{e}}^{t} + 1}.
> $$
> 
> 代入 $t = 0$ ,可得 ${\left. \frac{{\mathrm{d}}^{2}y}{\mathrm{\;d}{x}^{2}}\right| }_{t = 0} = \frac{2}{3}$ .