## 例5.8
### 题目
P119 已知函数 $y = y( x)$ 由方程 ${x}^{3} + {y}^{3} - {3x} + {3y} - 2 = 0$ 确定,求 $y( x)$ 的极值.
### 分析
直接隐函数求导然后判定就可以了
### 解
【解】方程 ${x}^{3} + {y}^{3} - {3x} + {3y} - 2 = 0$ 两边同时关于 $x$ 求一阶、二阶导数,分别为

$$
3{x}^{2} + 3{y}^{2}{y}^{\prime } - 3 + 3{y}^{\prime } = 0,
$$

①

$$
{6x} + {6y}{( {y}^{\prime }) }^{2} + 3{y}^{2}{y}^{\prime \prime } + 3{y}^{\prime \prime } = 0.
$$

②

在①式中,令 ${y}^{\prime } = 0$ ,得 $x = - 1$ 或 $x = 1$ .

当 $x$ 分别取 -1 和 1 时,由

$$
{x}^{3} + {y}^{3} - {3x} + {3y} - 2 = 0
$$

得

$$
y( {-1}) = 0, y( 1) = 1\text{.}
$$

将 $x = - 1, y( {-1}) = 0$ 及 ${y}^{\prime }( {-1}) = 0$ 代入②式得

$$
{y}^{\prime \prime }( {-1}) = 2\text{.}
$$

因为

$$
{y}^{\prime }( {-1}) = 0,{y}^{\prime \prime }( {-1}) > 0,
$$

所以 $y( {-1}) = 0$ 是 $y( x)$ 的极小值.

将 $x = 1, y( 1) = 1$ 及 ${y}^{\prime }( 1) = 0$ 代入②式得

$$
{y}^{\prime \prime }( 1) = - 1
$$

因为

$$
{y}^{\prime }( 1) = 0,{y}^{\prime \prime }( 1) < 0,
$$

所以 $y( 1) = 1$ 是 $y( x)$ 的极大值.