---
publish: true
tags: []
aliases: 
finished: true
title: 题3
created: "2024-10-04 13:54"
updated: "2024-12-11 05:17"
---
## 题3
### 题目
> [!question]+
> 设函数
> $$f( x)  = \{  {\begin{array}{ll}  - 1, & x < 0, \\  1, & x \geq  0, \end{array}g( x)  = \{  \begin{array}{ll} 2 - {ax}, & x \leq   - 1, \\  x, &  - 1 < x < 0,\text{ 若 }f( x)  + g( x) \text{ 在 }\mathrm{R}\text{ 上 } \\  x - b, & x \geq  0, \end{array}. }.$$
> 连续, 则 ( )
> (A)$a = 3, b = 1$
> (B)$a = 3, b = 2$
> (C)$a =  - 3, b = 1$
> (D)$a =  - 3, b = 2$
### 分析
> [!NOTE]+
> ![](https://img.hwenyi.live/202412111317033.webp)
### 解
> [!done]-
> $f(x), g(x)$都是分段函数, 考虑$f(x) + g(x)$的连续性时, 应考虑$f(x) + g(x)$在$f(x), g(x)$的分界点处的连续性. $f(x)$有一个分界点$x = 0$; $g(x)$有两个分界点$x = -1, x = 0$.
> 
> 解 当$x \leq -1$时, $f(x) + g(x) = -1 + (2 - ax) = 1 - ax$.
> 
> 当$-1 < x < 0$时, $f(x) + g(x) = -1 + x$.
> 
> 当$x \geq 0$时, $f(x) + g(x) = 1 + (x - b) = 1 - b + x$.
> 
> 于是, $f(x) + g(x) = \begin{cases} 1 - ax, & x \leq -1, \\ -1 + x, & -1 < x < 0, \\ 1 - b + x, & x \geq 0. \end{cases}$
> 
> 由于$f(x) + g(x)$在$\mathbb{R}$上连续, 故$f(x) + g(x)$在$x = -1$和$x = 0$处均连续.
> 
> 因为$\lim_{x \to -1^{+}}[f(x) + g(x)] = \lim_{x \to -1^{+}}(-1 + x) = -2$, 而$[f(x) + g(x)]|_{x = -1} = 1 + a$, 所以$1 + a = -2$, 即$a = -3$.
> 
> 又因为$\lim_{x \to 0^{-}}[f(x) + g(x)] = \lim_{x \to 0^{-}}(-1 + x) = -1$, 而$[f(x) + g(x)]|_{x = 0} = 1 - b$, 所以$1 - b = -1$, 即$b = 2$.
> 
> 因此, $a = -3, b = 2$.