## 例2.25
### 题目
P82 (仅数学一、数学三) 已知 ${\mathrm{e}}^{{a}_{n}} = {a}_{n} + {\mathrm{e}}^{{b}_{n}},{a}_{n} > 0$ ,且 $\mathop{\sum }\limits_{{n = 1}}^{\infty }{a}_{n}$ 收敛.
(1) 证明 $\mathop{\sum }\limits_{{n = 1}}^{\infty }\frac{{b}_{n}}{{a}_{n}}$ 收敛;
(2) 求 $\mathop{\lim }\limits_{{n \rightarrow \infty }}\frac{{b}_{n}}{{a}_{n}^{2}}$ .
### 分析
这个题的$b_{n}$的正负是可以确定的
- [01:29](https://www.bilibili.com/video/BV1Yw4m1a757?p=82&t=89.627321#t=01:29.63) 
### 解
(1)【证】因为 $\mathop{\sum }\limits_{{n = 1}}^{\infty }{a}_{n}$ 收敛,所以 $\mathop{\lim }\limits_{{n \rightarrow \infty }}{a}_{n} = 0$ ,又因为 ${\mathrm{e}}^{{a}_{n}} - {\mathrm{e}}^{{b}_{n}} = {a}_{n} > 0$ ,所以 ${a}_{n} > {b}_{n}$ .
由 ${\mathrm{e}}^{x} \geq x + 1$ ,知 ${\mathrm{e}}^{{a}_{n}} \geq {a}_{n} + 1$ ,所以 ${a}_{n} + 1 \leq {a}_{n} + {\mathrm{e}}^{{b}_{n}}$ ,故 ${\mathrm{e}}^{{b}_{n}} \geq 1$ ,即 ${b}_{n} \geq 0$ . 又
$$
{b}_{n} = \ln ( {{\mathrm{e}}^{{a}_{n}} - {a}_{n}}) ,
$$
所以
$$
\mathop{\lim }\limits_{{n \rightarrow \infty }}\frac{\frac{{b}_{n}}{{a}_{n}}}{{a}_{n}} = \mathop{\lim }\limits_{{n \rightarrow \infty }}\frac{\ln ( {{\mathrm{e}}^{{a}_{n}} - {a}_{n}}) }{{a}_{n}^{2}} = \mathop{\lim }\limits_{{n \rightarrow \infty }}\frac{{\mathrm{e}}^{{a}_{n}} - {a}_{n} - 1}{{a}_{n}^{2}} = \frac{1}{2}.
$$
因为 $\mathop{\sum }\limits_{{n = 1}}^{\infty }{a}_{n}$ 收敛,故 $\mathop{\sum }\limits_{{n = 1}}^{\infty }\frac{{b}_{n}}{{a}_{n}}$ 收敛.
(2)【解】由(1)得
$$
\mathop{\lim }\limits_{{n \rightarrow \infty }}\frac{{b}_{n}}{{a}_{n}^{2}} = \mathop{\lim }\limits_{{n \rightarrow \infty }}\frac{\frac{{b}_{n}}{{a}_{n}}}{{a}_{n}} = \frac{1}{2}.
$$