## 例2.24
### 题目
P81 (仅数学一、数学三) 已知 ${\mathrm{e}}^{{a}_{n}} = {a}_{n} + {\mathrm{e}}^{{a}_{n} + {b}_{n}},{a}_{n} > 0$ ,且 $\mathop{\sum }\limits_{{n = 1}}^{\infty }{a}_{n}$ 收敛.
(1) 证明 $\mathop{\sum }\limits_{{n = 1}}^{\infty }{b}_{n}$ 收敛;
(2) 求 $\mathop{\lim }\limits_{{n \rightarrow \infty }}\frac{{b}_{n}}{{a}_{n}}$ .
### 分析
这里是可以反解出来这个$b_{n}$的
- [01:50](https://www.bilibili.com/video/BV1Yw4m1a757?p=82&t=110.247795#t=01:50.25) 
### 解
(1)【证】令 ${a}_{n} + {b}_{n} = {c}_{n}$ ,则 ${c}_{n} = \ln ( {{\mathrm{e}}^{{a}_{n}} - {a}_{n}})$ . 由于 $\mathop{\sum }\limits_{{n = 1}}^{\infty }{a}_{n}$ 收敛,故 $\mathop{\lim }\limits_{{n \rightarrow \infty }}{a}_{n} = 0$ ,所以有 $\mathop{\lim }\limits_{{n \rightarrow \infty }}\frac{{c}_{n}}{{a}_{n}} = 0$ ,故
$\mathop{\sum }\limits_{{n = 1}}^{\infty }{c}_{n}$ 收敛,所以 $\mathop{\sum }\limits_{{n = 1}}^{\infty }{b}_{n}$ 收敛.
(2)【解】 $\mathop{\lim }\limits_{{n \rightarrow \infty }}\frac{{b}_{n}}{{a}_{n}} = \mathop{\lim }\limits_{{n \rightarrow \infty }}\frac{{a}_{n} + {b}_{n} - {a}_{n}}{{a}_{n}} = \mathop{\lim }\limits_{{n \rightarrow \infty }}\frac{{a}_{n} + {b}_{n}}{{a}_{n}} - 1 = \mathop{\lim }\limits_{{n \rightarrow \infty }}\frac{\ln ( {{\mathrm{e}}^{{a}_{n}} - {a}_{n}}) }{{a}_{n}} - 1 = 0 - 1 = - 1$ .
