## 例13.32
### 题目
P317 设函数$F( {a, b}) = {\int }_{a{b}^{-1}}^{ab}( {a - {bx}}) f( x) \mathrm{d}x, f( x)$可导,记${I}_{1} = {F}_{ab}( {1,1}) ,{I}_{2} = {F}_{ba}( {1, - 1})$,则( ).
(A)${I}_{1} > {I}_{2}$(B)${I}_{1} < {I}_{2}$(C)${I}_{1} = {I}_{2}$(D)${I}_{1}{I}_{2} > 0$
### 分析
本质上应该是莱布尼兹公式求导，有点超了，略过
### 解
![](https://img.hwenyi.tech/202410262012678.webp)
【解】应选(C).

$$
F( {a, b}) = a{\int }_{a{b}^{-1}}^{ab}f( x) \mathrm{d}x - b{\int }_{a{b}^{-1}}^{ab}{xf}( x) \mathrm{d}x,
$$

$$
{F}_{a}^{\prime } = {\int }_{a{b}^{-1}}^{ab}f( x) \mathrm{d}x + a\lbrack {{bf}( {ab}) - {b}^{-1}f( {a{b}^{-1}}) }\rbrack - b\lbrack {a{b}^{2}f( {ab}) - a{b}^{-2}f( {a{b}^{-1}}) }\rbrack
$$

$$
= {\int }_{a{b}^{-1}}^{ab}f( x) \mathrm{d}x + {abf}( {ab}) - a{b}^{3}f( {ab}) ,
$$

$$
{F}_{ab}^{\prime \prime } = \lbrack {{af}( {ab}) + \frac{a}{{b}^{2}}f( {a{b}^{-1}}) }\rbrack + {af}( {ab}) + {a}^{2}b{f}^{\prime }( {ab}) - {3a}{b}^{2}f( {ab}) - {a}^{2}{b}^{3}{f}^{\prime }( {ab}) .
$$

于是 ${F}_{ab}^{\prime \prime }( {1,1}) = 0,{F}_{ba}^{\prime \prime }( {1, - 1}) = {F}_{ab}^{\prime \prime }( {1, - 1}) = 0$ ,于是 ${I}_{1} = {I}_{2}$ . 故选(C).