---
publish: true
tags: 
aliases: 
finished: true
title: 例13.21
created: "2024-10-13 06:54"
updated: "2024-10-26 07:46"
---
## 例13.21
### 题目
P311 设$\frac{( {x + {ay}}) \mathrm{d}x + y\mathrm{\;d}y}{{( x + y) }^{2}}$是某个二元函数的全微分,求$a$的值.
### 分析
形如$Pdx+Qdy$这样的结构是[[全微分]]充要于$P_{ y} = Q_{ x}$，也就是$dx$这部分对y求导，$dy$这部分对x求导，交叉求导
### 解
![](https://img.hwenyi.tech/202410261546065.webp)
【解】记 $u( {x, y}) = \frac{x + {ay}}{{( x + y) }^{2}}, v( {x, y}) = \frac{y}{{( x + y) }^{2}}$ ,则
$$
\frac{\partial u( {x, y}) }{\partial y} = \frac{a{( x + y) }^{2} - 2( {x + {ay}}) ( {x + y}) }{{( x + y) }^{4}} = \frac{a( {x + y}) - 2( {x + {ay}}) }{{( x + y) }^{3}},
$$
$$
\frac{\partial v( {x, y}) }{\partial x} = - \frac{2y}{{( x + y) }^{3}}.
$$
依题意, $\frac{\partial u( {x, y}) }{\partial y} = \frac{\partial v( {x, y}) }{\partial x}$ ,即 $\frac{a( {x + y}) - 2( {x + {ay}}) }{{( x + y) }^{3}} = - \frac{2y}{{( x + y) }^{3}}$ ,所以 $( {a - 2}) x - {ay} = - {2y}$ . 故 $a = 2$ .
