---
publish: true
tags: 
aliases: 
finished: true
title: 题6
created: "2024-10-04 14:06"
updated: "2024-12-01 06:54"
---
## 题6
### 题目
> [!question]+
> 设函数 $f( {x, y})$ 可微,且 $f( {x + 1,{\mathrm{e}}^{x}}) = x{( x + 1) }^{2}, f( {x,{x}^{2}}) = 2{x}^{2}\ln x$ ,则 $\mathrm{d}f( {1,1}) = ( \;)$
> (A) $\mathrm{d}x + \mathrm{d}y$ . 
> (B) $\mathrm{d}x - \mathrm{d}y$ .
> (C) $\mathrm{d}y$ . 
> (D) $- \mathrm{d}y$ .
### 分析
> [!NOTE]+
> ![](https://img.hwenyi.tech/202412071920674.webp)
### 解
> [!done]-
> 解 根据全微分的定义,
> 
> $$
> \mathrm{d}f( {1,1}) = {f}_{1}^{\prime }( {1,1}) \mathrm{d}x + {f}_{2}^{\prime }( {1,1}) \mathrm{d}y.
> $$
> 
> 对 $f( {x + 1,{\mathrm{e}}^{x}}) = x{( x + 1) }^{2}, f( {x,{x}^{2}}) = 2{x}^{2}\ln x$ 两端均关于 $x$ 求导,可得
> 
> $$
> {f}_{1}^{\prime }( {x + 1,{\mathrm{e}}^{x}}) + {f}_{2}^{\prime }( {x + 1,{\mathrm{e}}^{x}}) \cdot {\mathrm{e}}^{x} = {( x + 1) }^{2} + x \cdot 2( {x + 1}) = ( {x + 1}) ( {{3x} + 1}) . \tag{1}
> $$
> 
> $$
> {f}_{1}^{\prime }( {x,{x}^{2}}) + {f}_{2}^{\prime }( {x,{x}^{2}}) \cdot {2x} = {4x}\ln x + 2{x}^{2} \cdot \frac{1}{x} = {2x}( {2\ln x + 1}) . \tag{2}
> $$
> 
> 在 $( 1)$ 式中令 $x = 0$ ,可得 ${f}_{1}^{\prime }( {1,1}) + {f}_{2}^{\prime }( {1,1}) = 1$ . 在 $( 2)$ 式中令 $x = 1$ ,可得 ${f}_{1}^{\prime }( {1,1}) +$ $2{f}_{2}^{\prime }( {1,1}) = 2$ . 联立两式解得 ${f}_{1}^{\prime }( {1,1}) = 0,{f}_{2}^{\prime }( {1,1}) = 1$ .
> 
> 因此, $\mathrm{d}f( {1,1}) = \mathrm{d}y$ . 应选 C.