---
publish: true
tags: []
aliases: 
finished: true
title: 题13
created: "2024-10-04 13:54"
updated: "2024-12-11 07:25"
---
## 题13
### 题目
> [!question]+
> 设函数 $z = z( {x, y})$ 由方程 $\ln z + {\mathrm{e}}^{z - 1} = {xy}$ 确定,则 ${. \frac{\partial z}{\partial x}| }_{( 2,\frac{1}{2}) } =$
### 分析
> [!NOTE]+
> ![](https://img.hwenyi.tech/202412111525405.webp)
### 解
> [!done]-
> (解) (法一) 对已知方程两端关于 $x$ 求导，可得
> 
> $\frac{1}{z} \cdot \frac{\partial z}{\partial x} + e^{z - 1} \cdot \frac{\partial z}{\partial x} = y$. (1)
> 
> 将 $x = 2, y = \frac{1}{2}$ 代入已知方程可得，$\ln z + e^{z - 1} = 1$。解得 $z = 1$。
> 
> 将 $x = 2, y = \frac{1}{2}, z = 1$ 代入(1)式可得，$2\frac{\partial z}{\partial x}\Bigr|_{(2,\frac{1}{2})} = \frac{1}{2}$，即 $\frac{\partial z}{\partial x}\Bigr|_{(2,\frac{1}{2})} = \frac{1}{4}$。
> 
> (法二) 记 $F(x, y, z) = \ln z + e^{z - 1} - xy$，则 $F_x'(x, y, z) = -y$，$F_z'(x, y, z) = \frac{1}{z} + e^{z - 1}$。
> 
> 将 $x = 2, y = \frac{1}{2}$ 代入已知方程可得，$\ln z + e^{z - 1} = 1$。解得 $z = 1$。
> 
> 根据隐函数存在定理，
> 
> $\frac{\partial z}{\partial x}\Bigr|_{(2,\frac{1}{2})} = -\frac{F_x'(2,\frac{1}{2},1)}{F_z'(2,\frac{1}{2},1)} = -\frac{-\frac{1}{2}}{2} = \frac{1}{4}$.